examples/sampler/common.v
@@ -35,14 +35,6 @@ Definition ge := ltac:(get_ge am_ge prog).
 
 Definition header_sample_t: P4Type := ltac:(get_type "header_sample_t" ge).
 Definition metadata_t: P4Type := ltac:(get_type "metadata_t" ge).
-Definition ingress_intrinsic_metadata_t: P4Type :=
-  ltac:(get_type "ingress_intrinsic_metadata_t" ge).
-Definition ingress_intrinsic_metadata_from_parser_t: P4Type :=
-  ltac:(get_type "ingress_intrinsic_metadata_from_parser_t" ge).
-Definition ingress_intrinsic_metadata_for_deparser_t: P4Type :=
-  ltac:(get_type "ingress_intrinsic_metadata_for_deparser_t" ge).
-Definition ingress_intrinsic_metadata_for_tm_t: P4Type :=
-  ltac:(get_type "ingress_intrinsic_metadata_for_tm_t" ge).
 Definition tcp_h: P4Type := ltac:(get_type "tcp_h" ge).
 Definition udp_h: P4Type := ltac:(get_type "udp_h" ge).
 Definition ipv4_h: P4Type := ltac:(get_type "ipv4_h" ge).
