examples/sampler/verif_sampler_ingress_deparser.v
@@ -1,0 +1,42 @@
+Require Import ProD3.core.PacketFormat.
+Require Import Poulet4.P4light.Syntax.P4defs.
+Require Import Poulet4.P4light.Semantics.Semantics.
+Require Import ProD3.core.Core.
+Require Import Poulet4.P4light.Architecture.Tofino.
+Require Import ProD3.core.Tofino.
+Require Import ProD3.examples.sampler.ModelRepr.
+Require Import ProD3.examples.sampler.common.
+Require Import ProD3.core.ProgNotations.
+Require Import Poulet4.P4light.Syntax.P4Notations.
+Require Import Hammer.Plugin.Hammer.
+Require Export Coq.Program.Program.
+Import ListNotations.
+
+Definition p := ["pipe"; "ingress_deparser"].
+
+Definition deparser_fundef :=
+  ltac:(get_fd ["SwitchIngressDeparser"; "apply"] ge).
+
+Definition deparser_spec: func_spec :=
+  WITH,
+    PATH p
+    MOD None [["packet_out"]]
+    WITH (pout : packet_out) hdr ig_md ig_intr_dpprsr_md
+         (_: ⊢ᵥ hdr \: header_sample_t),
+      PRE
+        (ARG [eval_val_to_sval hdr; ig_md; ig_intr_dpprsr_md]
+        (MEM []
+        (EXT [ExtPred.singleton ["packet_out"] (ObjPout pout)])))
+      POST
+        (ARG_RET [eval_val_to_sval hdr] ValBaseNull
+           (MEM []
+              (EXT [ExtPred.singleton ["packet_out"]
+                      (ObjPout (pout ++ encode hdr))]))).
+
+Lemma parser_start_body:
+  func_sound ge deparser_fundef nil deparser_spec.
+Proof.
+  start_function.
+  step_call (@packet_out_emit_body Info); [entailer | eapply emit_encode; eauto|].
+  step. entailer.
+Qed.
